writeback for cache cleaning

examples/scache/Cache.i.dfy
@@ -2,16 +2,19 @@ include "AtomicRefcount.i.dfy"
 include "AtomicStatus.i.dfy"
 include "AtomicIndexLookup.i.dfy"
 include "ArrayPtr.s.dfy"
+include "DiskIO.i.dfy"
 
 module CacheImpl {
   import opened Constants
   import opened AtomicStatusImpl
   import opened AtomicRefcountImpl
   import opened AtomicIndexLookupImpl
+  import opened AtomicSpec
   import opened LinearMaybe
   import opened Ptrs
   import opened NativeTypes
   import opened Options
+  import DiskIO
 
   datatype Cache = Cache(
     data: seq<Ptr>,
@@ -20,23 +23,25 @@ module CacheImpl {
     status: seq<AtomicStatus>,
     read_refcounts: seq<seq<AtomicRefcount>>,
 
-    cache_idx_of_page: seq<AtomicIndexLookup>
+    cache_idx_of_page: seq<AtomicIndexLookup>,
+
+    global_clockpointer: Atomic<uint32, NullGhostType>
   )
 
   predicate Inv(c: Cache)
   {
-    && |c.data| == CacheSize()
-    && |c.disk_idx_of_entry| == CacheSize()
-    && |c.status| == CacheSize()
-    && (forall i | 0 <= i < CacheSize() ::
+    && |c.data| == CACHE_SIZE
+    && |c.disk_idx_of_entry| == CACHE_SIZE
+    && |c.status| == CACHE_SIZE
+    && (forall i | 0 <= i < CACHE_SIZE ::
        atomic_status_inv(c.status[i], c.data[i]))
-    && |c.read_refcounts| == NThreads()
-    && (forall j | 0 <= j < NThreads() ::
-        |c.read_refcounts[j]| == CacheSize())
-    && (forall j, i | 0 <= j < NThreads() && 0 <= i < CacheSize() ::
+    && |c.read_refcounts| == NUM_THREADS
+    && (forall j | 0 <= j < NUM_THREADS ::
+        |c.read_refcounts[j]| == CACHE_SIZE)
+    && (forall j, i | 0 <= j < NUM_THREADS && 0 <= i < CACHE_SIZE ::
         atomic_refcount_inv(c.read_refcounts[j][i], c.data[i], j))
-    && |c.cache_idx_of_page| == NDiskPages()
-    && (forall d | 0 <= d < NDiskPages() ::
+    && |c.cache_idx_of_page| == NUM_DISK_PAGES
+    && (forall d | 0 <= d < NUM_DISK_PAGES ::
         atomic_index_lookup_inv(c.cache_idx_of_page[d], d))
   }
 
@@ -49,10 +54,11 @@ module CacheImpl {
     predicate is_handle(c: Cache, cache_idx: int)
     requires Inv(c)
     {
-      && 0 <= cache_idx < CacheSize()
+      && 0 <= cache_idx < CACHE_SIZE
       && data.ptr == c.data[cache_idx]
       && idx.ptr == c.disk_idx_of_entry[cache_idx]
       && cache_entry == CacheResources.CacheEntry(Some(idx.v), cache_idx, data.s)
+      && |data.s| == 4096
     }
 
     predicate is_page_handle(c: Cache, disk_idx: int)
@@ -64,10 +70,36 @@ module CacheImpl {
     }
   }
 
+  linear datatype CacheEntryReadOnlyHandle = CacheEntryReadOnlyHandle(
+      linear cache_entry: CacheResources.R, // TODO should be readonly
+      linear data: ConstArrayDeref<byte>,
+      linear idx: ConstDeref<int>
+  )
+  {
+    predicate is_handle(c: Cache, cache_idx: int)
+    requires Inv(c)
+    {
+      && 0 <= cache_idx < CACHE_SIZE
+      && data.ptr == c.data[cache_idx]
+      && idx.ptr == c.disk_idx_of_entry[cache_idx]
+      && cache_entry == CacheResources.CacheEntry(Some(idx.v), cache_idx, data.s)
+      && |data.s| == 4096
+    }
+
+    predicate is_page_handle(c: Cache, disk_idx: int)
+    requires Inv(c)
+    {
+      && cache_entry.CacheEntry?
+      && is_handle(c, cache_entry.cache_idx)
+      && cache_entry.disk_idx_opt == Some(disk_idx)
+    }
+  }
+
+
   method take_write_lock_on_cache_entry(c: Cache, cache_idx: int)
   returns (linear handle: CacheEntryHandle)
   requires Inv(c)
-  requires 0 <= cache_idx < CacheSize()
+  requires 0 <= cache_idx < CACHE_SIZE
   ensures handle.is_handle(c, cache_idx)
   decreases *
   {
@@ -102,8 +134,8 @@ module CacheImpl {
     }
 
     var j := 0;
-    while j < NThreads()
-    invariant 0 <= j <= NThreads()
+    while j < NUM_THREADS
+    invariant 0 <= j <= NUM_THREADS
     invariant w == 
         ReadWriteLockResources.WritePending(c.data[cache_idx], j)
     {
@@ -132,7 +164,7 @@ module CacheImpl {
   method release_write_lock_on_cache_entry(c: Cache, cache_idx: int,
       linear handle: CacheEntryHandle)
   requires Inv(c)
-  requires 0 <= cache_idx < CacheSize()
+  requires 0 <= cache_idx < CACHE_SIZE
   requires handle.is_handle(c, cache_idx)
 
   /*method take_write_lock_on_disk_entry(c: Cache, disk_idx: int)
@@ -141,10 +173,51 @@ module CacheImpl {
     
   }*/
 
+  method get_next_chunk(c: Cache)
+  requires Inv(c)
+  {
+    var l: uint32 := fetch_add(c.global_clockpointer, 1);
+    l := l % (NUM_CHUNKS as uint32);
+    var ci: uint32 := (l + CLEAN_AHEAD as uint32) % (NUM_CHUNKS as uint32);
+
+    var i: uint32 := 0;
+    while i < CHUNK_SIZE as uint32
+    {
+      var cache_idx := ci * (CHUNK_SIZE as uint32) + i;   
+
+      linear var write_back_r;
+      var do_write_back;
+      do_write_back, write_back_r :=
+          try_acquire_writeback(c.status[cache_idx], c.data[cache_idx]);
+
+      if do_write_back {
+        linear var readonly_handle: CacheEntryReadOnlyHandle :=
+            AtomicRefcountImpl.unsafe_obtain(); // TODO
+        assume readonly_handle.is_handle(c, cache_idx as int);
+
+        linear var CacheEntryReadOnlyHandle(
+            cache_entry, data, idx) := readonly_handle;
+
+        var disk_idx := ptr_const_read(c.disk_idx_of_entry[cache_idx], idx);
+        assume 0 <= disk_idx as int < NUM_DISK_PAGES;
+
+        linear var wgs := DiskIO.WritebackGhostState(
+            unwrap(write_back_r), cache_entry, idx);
+
+        DiskIO.disk_writeback_async(disk_idx as uint64, c.data[cache_idx],
+            data, wgs);
+      } else {
+        var _ := discard(write_back_r);
+      }
+
+      i := i + 1;
+    }
+  }
+
   method try_take_write_lock_disk_page(c: Cache, disk_idx: int)
   returns (success: bool, linear handle_out: maybe<CacheEntryHandle>)
   requires Inv(c)
-  requires 0 <= disk_idx < NDiskPages()
+  requires 0 <= disk_idx < NUM_DISK_PAGES
   ensures !success ==> handle_out == empty()
   ensures success ==> has(handle_out) &&
       peek(handle_out).is_page_handle(c, disk_idx)
@@ -172,3 +245,4 @@ module CacheImpl {
     }
   }
 }
+
