examples/scache/Constants.i.dfy
@@ -1,5 +1,9 @@
 module Constants {
-  function method NThreads() : int { 24 }
-  function method CacheSize() : int { 1048576 }
-  function method NDiskPages() : int { 536870912 }
+  const NUM_THREADS := 24;
+  const CACHE_SIZE := 1048576;
+  const NUM_DISK_PAGES := 536870912;
+
+  const CHUNK_SIZE := 64;
+  const NUM_CHUNKS := CACHE_SIZE / 64;
+  const CLEAN_AHEAD := NUM_CHUNKS / 3;
 }
